src/Backends/Boogie/Plugin.dfy
@@ -1,0 +1,52 @@
+include "../../AST/Translator.dfy"
+include "../../Interop/CSharpDafnyASTModel.dfy"
+include "../../Interop/CSharpDafnyInterop.dfy"
+include "../../Interop/CSharpInterop.dfy"
+include "../../Interop/StrTree.dfy"
+include "../../Passes/EliminateNegatedBinops.dfy"
+include "../../Transforms/BottomUp.dfy"
+include "../../Utils/Library.dfy"
+include "Compiler.dfy"
+
+module {:options "-functionSyntax:4"} {:extern "Bootstrap.Backends.Boogie.Interface"}
+  Bootstrap.Backends.Boogie.Interface
+{
+  import Interop.CSharpDafnyASTModel
+  import opened Interop.CSharpDafnyInterop
+  import opened Microsoft.Dafny
+  import Utils.StrTree
+  import StrTreeInterop = Interop.StrTree
+  import AST.Predicates
+  import AST.Translator
+  import Transforms.BottomUp
+  import Passes.EliminateNegatedBinops
+  import opened AST.Predicates.Deep
+  import Compiler
+
+  class {:extern} DafnyBoogieCompiler {
+    constructor() {
+    }
+
+    method Compile(dafnyProgram: CSharpDafnyASTModel.Program,
+                   wr: ConcreteSyntaxTree) {
+      var st := new StrTreeInterop.SyntaxTreeAdapter(wr);
+      match Translator.TranslateProgram(dafnyProgram) {
+        case Success(translated) =>
+          var tree := Compiler.Compile(translated);
+          st.WriteTree(tree);
+        case Failure(err) => // FIXME return an error
+          st.Write("!! Translation error: " + err.ToString());
+      }
+      st.Write("\n");
+    }
+
+    method EmitCallToMain(mainMethod: CSharpDafnyASTModel.Method,
+                          baseName: System.String,
+                          wr: ConcreteSyntaxTree) {
+      // var st := new SyntaxTreeAdapter(wr);
+      // var sClass := st.NewBlock("class __CallToMain");
+      // var sBody := sClass.NewBlock("public static void Main(string[] args)");
+      // sBody.WriteLine("DafnyRuntime.Helpers.WithHaltHandling(_module.Main);");
+    }
+  }
+}
