src/Interop/StrTree.dfy
@@ -1,0 +1,44 @@
+include "../Utils/StrTree.dfy"
+include "../Interop/CSharpDafnyInterop.dfy"
+
+module Bootstrap.Interop.StrTree {
+  import opened Utils.StrTree
+  import opened CSharpDafnyInterop
+  import Microsoft
+
+  class SyntaxTreeAdapter {
+    var wr: Microsoft.Dafny.ConcreteSyntaxTree
+
+    constructor(wr: Microsoft.Dafny.ConcreteSyntaxTree) {
+      this.wr := wr;
+    }
+
+    method Write(value: string) {
+      wr.Write(StringUtils.ToCString(value));
+    }
+
+    method WriteLine(value: string) {
+      wr.WriteLine(StringUtils.ToCString(value));
+    }
+
+    method NewBlock(header: string) returns (st': SyntaxTreeAdapter) {
+      var wr' := wr.NewBlock(StringUtils.ToCString(header));
+      st' := new SyntaxTreeAdapter(wr');
+    }
+
+    method WriteTree(tree: StrTree.StrTree) {
+      match tree {
+        case Str(s) =>
+          Write(s);
+        case SepSeq(sep, trees) =>
+          for i := 0 to |trees| {
+            if i != 0 && sep.Some? {
+              Write(sep.value);
+            }
+            WriteTree(trees[i]);
+          }
+        case Unsupported() =>
+      }
+    }
+  }
+}
